\documentclass[a4paper,12pt]{article}
\usepackage{amsmath,amsthm,amssymb}
\begin{document}

7. Prove that for any natural number $n$ $$2 + 2^2 + 2^3 + .. + 2^n = 2^{n+1} - 2$$

\begin{proof}

  Proof by induction. Base case for $n = 1$:

  \begin{align*}
    2^1 &= 2^{1+1} - 2 \\
        &= 2^2 - 2 \\
        &= 4 - 2 \\
        &= 2
  \end{align*} 

  Substituting $n + 1$, we get:

  \begin{align*}
    LHS &= 2 + 2^2 + 2^3 + .. + 2^{n+1} \\
        &= 2 + 2^2 + 2^3 + .. + 2^n + 2^{n+1} \tag{show second to last term} \\
        &= (2 + 2^2 + 2^3 + .. + 2^n) + 2^{n+1} \tag{group first terms} \\
        &= (2^{n+1} - 2) + 2^{n+1} \tag{by inductive statement} \\
        &= 2^{n+1} + 2^{n+1} - 2 \tag{re-arrange terms} \\
        &= 2(2^{n+1}) - 2 \tag{group similar terms} \\
        &= 2^{n+2} - 2 \\
        &= 2^{(n+1)+1} - 2 \\
        &= RHS
  \end{align*} 

\end{proof}

\end{document}
